In-depth cleanup of Model.AEAD.fsti and a work-in-progress implementation

src/Model.AEAD.fsti
@@ -4,250 +4,209 @@ module HS = FStar.HyperStack
 module I = Model.Indexing
 module U32 = FStar.UInt32
 module U128 = FStar.UInt128
-module M = LowStar.Modifies
+module B = LowStar.Buffer
+module Spec = Spec.Agile.AEAD
 
-open FStar.Bytes
-open FStar.UInt32
+#set-options "--fuel 0 --ifuel 0"
+
 open Mem
 
-type id = I.ae_id
-type alg = I.ea
+/// Abbreviations for idealization
+/// ------------------------------
 
-let is_safe i = I.ideal_AEAD && I.is_ae_honest i
-type safeid = i:id{is_safe i}
-type unsafeid = i:id{not (is_safe i)}
+// In this module, id is an AEAD id.
+let id = I.ae_id
 
-let ivlen (alg:alg) = 12ul
-let taglen = 16ul
+// ea = encryption alg
+let alg = I.ea
 
-let iv (alg:alg) =
-  let open FStar.Mul in
-  n:U128.t { U128.v n < pow2 (8 * v (ivlen alg)) }
+let is_safe i =
+  I.ideal_AEAD && I.is_ae_honest i
 
-let aadmax =
-  assert_norm (2000 <= pow2 32 - 1);
-  2000ul // arbitrary; enough for TLS
+let safe_id =
+  i:id{is_safe i}
 
-type aadlen_32 = l:U32.t {l <=^ aadmax}
-type plainLen = l:nat{l + v taglen < pow2 32}
-type plainLenMin (lmin:plainLen) = l:plainLen{l >= lmin}
+let unsafe_id =
+  i:id{~ (is_safe i)}
 
-noeq type plain_pkg (idt:eqtype) (safe:idt->bool) =
+/// Some redefinitions, using Spec
+/// ------------------------------
+
+// Not modeling arbitrary-length IVs as supported by AES-GCM.
+let iv_len (a: alg) =
+  12ul
+
+// Trying to follow the Fournet-Protzenko conventions: _len for machine lengths,
+// _length for spec (nat) lengths.
+let tag_len: x:U32.t { forall (a: alg). {:pattern Spec.tag_length a} U32.v x == Spec.tag_length a } =
+  16ul
+
+// JP: don't understand why this previously was UInt128.t -- remnant from
+// ancient code?
+let iv (a: alg) =
+  Spec.iv a
+
+// JP: this duplicates a fair amount of definitions from Spec.Agile.AEAD, but
+// here the bounds are tighter and force plain texts to not overflow 32 bits
+// once encrypted and tagged.
+//
+// TODO: it would be good to get everyone on the same page rather than duplicating things
+type plain_length = l:nat{l + U32.v tag_len < pow2 32}
+type plain_length_at_least (lmin: plain_length) = l:plain_length{lmin <= l}
+
+/// Packages, info (?)
+/// ------------------
+
+noeq
+type plain_pkg (idt: eqtype) (safe: idt -> bool) =
   | PlainPkg:
-    min_len: plainLen ->
-    plain: (i:idt -> plainLenMin min_len -> eqtype) ->
-    as_bytes: (i:idt -> l:plainLenMin min_len -> plain i l -> GTot (lbytes l)) ->
-    repr: (i:idt{not (safe i)} -> l:plainLenMin min_len -> p:plain i l -> Tot (b:lbytes l{b == as_bytes i l p})) ->
+    min_len: plain_length ->
+    plain: (i:idt -> plain_length_at_least min_len -> eqtype) ->
+    as_bytes: (i:idt -> l:plain_length_at_least min_len -> plain i l -> GTot (Spec.lbytes l)) ->
+    repr: (i:idt{not (safe i)} -> l:plain_length_at_least min_len -> p:plain i l -> Tot (b:Spec.lbytes l{b == as_bytes i l p})) ->
     plain_pkg idt safe
 
-noeq type nonce_pkg (idt:eqtype) (safe:idt->bool) (alg:idt->GTot I.ea) =
+noeq
+type nonce_pkg (idt: eqtype) (safe: idt -> bool) (alg: idt -> GTot I.ea) =
   | NoncePkg:
-    nonce: (i:idt -> t:Type0{hasEq t}) ->
+    nonce: (i:idt -> eqtype) ->
     as_bytes: (i:idt -> nonce i -> GTot (iv (alg i))) ->
-    repr: (i:idt{not (safe i)} -> n:nonce i -> Tot (r:iv (alg i){r == as_bytes i n})) ->
+    repr: (i:idt{not (safe i)} -> n:nonce i -> Tot (r:iv (alg i) {r == as_bytes i n})) ->
     nonce_pkg idt safe alg
 
 noeq type info' = {
   alg: alg;
+  // JP: subq is an abbreviation that means "sub quic region"
   region: r:subq{r `HS.disjoint` q_ae_region};
   plain: plain_pkg id is_safe;
   nonce: nonce_pkg id is_safe I.ae_id_ginfo;
 }
 
-type info (i:id) =
+let info (i:id) =
   info:info'{I.ae_id_ginfo i == info.alg}
 
-let plainLenM (#i:id) (u:info i) = plainLenMin (PlainPkg?.min_len u.plain)
+/// Accessors for info
+/// ------------------
 
-let plain (#i:id) (u:info i) (l:plainLenM u) =
+// Accessor for the info type.
+let at_least (#i:id) (u:info i) =
+  plain_length_at_least (PlainPkg?.min_len u.plain)
+
+let plain (#i:id) (u:info i) (l: at_least u) =
   (PlainPkg?.plain u.plain) i l
- 
-let plain_as_bytes (#i:id) (#u:info i) (#l:plainLenM u) (p:plain u l) : GTot (lbytes l) = 
+
+let plain_as_bytes (#i:id) (#u:info i) (#l:at_least u) (p:plain u l) : GTot (Spec.lbytes l) =
   (PlainPkg?.as_bytes u.plain) i l p
-  
-let plain_repr (#i:unsafeid) (#u:info i) (#l:plainLenM u) (p:plain u l) : Tot (r:lbytes l{r == plain_as_bytes p}) =
+
+let plain_repr (#i: unsafe_id) (#u:info i) (#l:at_least u) (p:plain u l) : Tot (r:Spec.lbytes l{r == plain_as_bytes p}) =
   (PlainPkg?.repr u.plain) i l p
 
-//let nonce_tag (#i:I.id) (u:info i) : t:Type0{hasEq t} = NoncePkg?.tag u.nonce
+let nonce (#i:id) (u:info i) =
+  NoncePkg?.nonce u.nonce i
 
-let nonce (#i:id) (u:info i) : t:Type0{hasEq t} = NoncePkg?.nonce u.nonce i
-val keylen : #i:id -> u:info i -> U32.t
-val statelen : #i:id -> u:info i -> U32.t
+/// Plains, ciphers and entries in the log
+/// --------------------------------------
 
-type cipher (i:id) (u:info i) (l:plainLenM u) =
-  lbytes (l + (UInt32.v taglen))
+let cipher (#i:id) (u:info i) (l:at_least u) =
+  Spec.lbytes (l + UInt32.v tag_len)
 
-type cipher32 (i:id) (l:U32.t{UInt.size (v l + 16) 32}) = lbytes32 (l +^ taglen)
+let ad #i (u: info i) =
+  Spec.ad u.alg
 
-type adata = b:bytes{length b <= v aadmax}
-
+noeq
 type entry (i:id) (u:info i) =
   | Entry:
     n: nonce u ->
-    ad: adata ->
-    #l: plainLenM u ->
+    ad: ad u ->
+    #l: at_least u ->
     p: plain u l ->
-    c: cipher i u l ->
+    c: cipher u l ->
     entry i u
 
-val aead_writer: i:id -> Type0
-val aead_reader: #i:id -> w:aead_writer i -> Type0
+/// Readers & writers
+/// -----------------
+
+val aead_writer: i:id -> Type u#1
+val aead_reader: #i:id -> w:aead_writer i -> Type u#1
 
 val wgetinfo: #i:id -> aead_writer i -> Tot (info i)
 val rgetinfo: #i:id -> #w:aead_writer i -> aead_reader w -> Tot (u:info i{u == wgetinfo w})
 
-val wlog: #i:safeid -> w:aead_writer i -> mem -> GTot (Seq.seq (entry i (wgetinfo w)))
-let rlog (#i:safeid) (#w: aead_writer i) (r:aead_reader w) (h:mem) = wlog w h
+val wlog: #i:safe_id -> w:aead_writer i -> mem -> GTot (Seq.seq (entry i (wgetinfo w)))
+let rlog (#i:safe_id) (#w: aead_writer i) (r:aead_reader w) (h:mem) = wlog w h
 
-val footprint: #i:id -> aead_writer i -> l:M.loc{l `M.loc_disjoint` loc_ae_region ()}
-val wfootprint: #i:id -> aead_writer i -> M.loc
-
-//Leaving this abstract for now; but it should imply Crypto.AEAD.Invariant.safelen i len (otp_offset i)
-val safelen: id -> nat -> GTot bool
-let ok_plain_len_32 (i:id) = l:U32.t{safelen i (v l)}
+// JP: disjointness? anything?
+val wfootprint: #i:id -> aead_writer i -> GTot B.loc
 
 val winvariant : #i:id -> aead_writer i -> mem -> Type0
 //let rinvariant (#i:I.id) (#w:aead_writer i) (r:aead_reader w) (h:mem) =
 //  winvariant w h
 
-val wframe_invariant: #i:id -> w:aead_writer i -> h0:mem -> l:M.loc -> h1:mem ->
+val wframe_invariant: #i:id -> l:B.loc -> w:aead_writer i -> h0:mem -> h1:mem ->
   Lemma
-    (requires (winvariant w h0 /\
-      M.modifies l h0 h1 /\
-      M.loc_disjoint l (wfootprint w)))
-    (ensures winvariant w h1)
+    (requires (
+      winvariant w h0 /\
+      B.modifies l h0 h1 /\
+      B.loc_disjoint l (wfootprint w)))
+    (ensures
+      winvariant w h1)
 
-val frame_log: #i:safeid -> w:aead_writer i -> log:Seq.seq (entry i (wgetinfo w)) ->
-  h0:mem -> l:M.loc -> h1:mem ->
+val frame_log: #i:safe_id -> l:B.loc -> w:aead_writer i -> h0:mem -> h1:mem ->
   Lemma
     (requires
-      wlog w h0 == log /\
-      M.modifies l h0 h1 /\
-      M.loc_disjoint l (wfootprint w))
-    (ensures wlog w h1 == log)
+      winvariant w h0 /\
+      B.modifies l h0 h1 /\
+      B.loc_disjoint l (wfootprint w))
+    (ensures wlog w h1 == wlog w h0)
 
-(*** The main stateful API ***)
+/// Main stateful API
+/// -----------------
 
 (** Allocating a writer **)
 val gen (i:id) (u:info i) : ST (aead_writer i)
   (requires (fun h -> True))
-  (ensures  (fun h0 w h1 ->
+  (ensures (fun h0 w h1 ->
+    winvariant w h1 /\
+
+    B.modifies B.loc_none h0 h1 /\
+    B.fresh_loc (wfootprint w) h0 h1 /\
+    B.(loc_includes (loc_ae_region ()) (wfootprint w)) /\
+
     wgetinfo w == u /\
-    M.modifies M.loc_none h0 h1 /\ // allocates only
-    wfootprint w == loc_ae_region () /\
-    (I.ideal_AEAD && I.is_ae_honest i ==> wlog w h1 == Seq.empty) /\
-     winvariant w h1
-   ))
+    (I.ideal_AEAD && I.is_ae_honest i ==> wlog w h1 == Seq.empty)))
 
 (** Building a reader from a writer **)
-
-val genReader (#i: id) (w: aead_writer i) : ST (aead_reader w)
+val gen_reader (#i: id) (w: aead_writer i) : ST (aead_reader w)
   (requires (fun h -> winvariant w h))
-  (ensures  (fun h0 r h1 ->
-    M.modifies M.loc_none h0 h1 /\
-    winvariant w h1)
+  (ensures (fun h0 r h1 ->
+    // JP: can this be strengthened into h0 == h1?
+    B.modifies B.loc_none h0 h1)
   )
-
-(*
-(** [coerce]: Only needed for modeling the adversary *)
-val coerce
-         (i: I.id)
-       (rgn: eternal_region)
-       (key: lbuffer (v (keylen i)))
-      : ST  (aead_state i I.Writer)
-  (requires (fun h ->
-             ~ (Flag.prf i) /\
-             Buffer.live h key))
-  (ensures  (fun h0 st h1 ->
-               HS.modifies Set.empty h0 h1 /\
-               invariant st h1))
-
-
-(** [leak]: Only needed for modeling the adversary *)
-val leak
-      (#i: I.id)
-      (st: aead_state i I.Writer)
-    : ST (lbuffer (v (statelen i)))
-  (requires (fun _ -> ~(Flag.prf i)))
-  (ensures  (fun h0 _ h1 ->
-               HS.modifies Set.empty h0 h1 /\
-               invariant st h1))
-
-
-// enc_dec_separation: Calling AEAD.encrypt/decrypt requires this separation
-let enc_dec_separation (#i:_) (#rw:_) (st:aead_state i rw)
-                       (#aadlen:nat) (aad: lbuffer aadlen)
-                       (#plainlen:nat) (plain: Plain.plainBuffer i plainlen)
-                       (#cipherlen: nat) (cipher:lbuffer cipherlen) =
-    Buffer.disjoint aad cipher /\
-    Buffer.disjoint (Plain.as_buffer plain) aad /\
-    Buffer.disjoint (Plain.as_buffer plain) cipher /\
-    HS.disjoint_regions (Set.as_set [Buffer.frameOf (Plain.as_buffer plain);
-                                     Buffer.frameOf cipher;
-                                     Buffer.frameOf aad])
-                        (Set.as_set [log_region st;
-                                     prf_region st]) /\
-    Buffer.frameOf cipher <> HS.root /\
-    Buffer.frameOf aad <> HS.root /\
-    Buffer.frameOf (Plain.as_buffer plain) <> HS.root
-    (* is_eternal_region (Buffer.frameOf cipher) /\ // why? *)
-    (* is_eternal_region (Buffer.frameOf (Plain.as_buffer plain)) /\ //why? *)
-    (* is_eternal_region (Buffer.frameOf aad) /\ //why? *)
-
-let enc_dec_liveness (#i:_) (#rw:_) (st:aead_state i rw)
-                     (#aadlen:nat) (aad: lbuffer aadlen)
-                     (#plainlen:nat) (plain: Plain.plainBuffer i plainlen)
-                     (#cipherlen: nat) (cipher:lbuffer cipherlen) (h:mem) =
-    let open HS in
-    Buffer.live h aad /\
-    Buffer.live h cipher /\
-    Plain.live h plain /\
-    log_region st `is_in` h.h /\
-    prf_region st `is_in` h.h
-
-let entry_of
-          (#i: I.id)
-           (n: iv (I.cipherAlg_of_id i))
-     (#aadlen: aadlen_32)
-         (aad: lbuffer (v aadlen))
-   (#plainlen: ok_plain_len_32 i)
-       (plain: Plain.plainBuffer i (v plainlen))
-  (cipher_tag: lbuffer (v plainlen + v taglen))
-           (h: mem) : GTot (entry i) =
-  let aad = Buffer.as_seq h aad in
-  let p = Plain.sel_plain h plainlen plain in
-  let c = Buffer.as_seq h cipher_tag in
-  mk_entry n aad p c
-*)
 
 let nonce_filter (#i:id) (#w:aead_writer i) (n:nonce (wgetinfo w)) (e:entry i (wgetinfo w)) : bool =
   Entry?.n e = n
 
-let wentry_for_nonce (#i:safeid) (w:aead_writer i) (n:nonce (wgetinfo w)) (h:mem)
+let wentry_for_nonce (#i:safe_id) (w:aead_writer i) (n:nonce (wgetinfo w)) (h:mem)
   : GTot (option (entry i (wgetinfo w))) =
   Seq.find_l (nonce_filter #i #w n) (wlog w h)
 
-let fresh_nonce (#i:safeid) (w:aead_writer i) (n:nonce (wgetinfo w)) (h:mem)
+let fresh_nonce (#i:safe_id) (w:aead_writer i) (n:nonce (wgetinfo w)) (h:mem)
   : GTot bool =
   None? (wentry_for_nonce w n h)
-
-(*let just_one_buffer (#a:Type) (b:Buffer.buffer a) : GTot fp =
-   as_set [(Buffer.frameOf b, SomeRefs (as_set [Buffer.as_addr b]))]
-*)
 
 val encrypt
   (i: id)
   (w: aead_writer i)
   (n: nonce (wgetinfo w))
-  (aad: adata)
-  (l: plainLenM (wgetinfo w))
+  (aad: ad (wgetinfo w))
+  (l: at_least (wgetinfo w))
   (p: plain (wgetinfo w) l)
-  : ST (cipher i (wgetinfo w) l)
+  : ST (cipher (wgetinfo w) l)
   (requires (fun h0 ->
     winvariant w h0 /\
     (is_safe i ==> fresh_nonce w n h0)))
   (ensures (fun h0 c h1 ->
-    M.modifies (wfootprint w) h0 h1 /\
+    B.modifies (wfootprint w) h0 h1 /\
     winvariant w h1 /\
     (is_safe i ==>
       wlog w h1 == Seq.snoc (wlog w h0) (Entry n aad p c))))
@@ -256,22 +215,23 @@ val decrypt
   (i: id)
   (#w: aead_writer i)
   (r: aead_reader w)
-  (aad:adata)
+  (aad: ad (wgetinfo w))
   (n: nonce (rgetinfo r))
-  (l:plainLenM (wgetinfo w))
-  (c:cipher i (wgetinfo w) l)
+  (l:at_least (wgetinfo w))
+  (c:cipher (wgetinfo w) l)
   : ST (option (plain (rgetinfo r) l))
   (requires (fun h0 ->
     winvariant w h0))
   (ensures fun h0 res h1 ->
     winvariant w h1 /\
-    M.modifies M.loc_none h0 h1 /\
+    B.modifies B.loc_none h0 h1 /\
     (is_safe i ==>
       (match wentry_for_nonce w n h0 with
       | None -> None? res
       | Some (Entry _ aad' #l' p' c') ->
-        (if aad' = aad && c' = c && l = l' then res = Some p'
-        else None? res)
+        let matches = aad' == aad /\ c' == c /\ l == l' in
+        (matches ==> res = Some p') /\
+        (~matches ==> res = None)
       )
     )
   )
