src/Model.AEAD.fst
@@ -1,0 +1,68 @@
+module Model.AEAD
+
+module HS = FStar.HyperStack
+module I = Model.Indexing
+module U32 = FStar.UInt32
+module U128 = FStar.UInt128
+module B = LowStar.Buffer
+module Spec = Spec.Agile.AEAD
+
+#set-options "--fuel 0 --ifuel 0"
+
+open Mem
+
+let log #i (u: info i): Type0 =
+  if is_safe i then
+    Seq.seq (entry i u)
+  else
+    unit
+
+let model_writer i =
+  u:info i & B.pointer (log #i u)
+
+let aead_writer (i: id): Type u#1 =
+  if is_safe i then
+    model_writer i
+  else
+    info i
+
+let aead_reader #i (w: aead_writer i): Type u#1 =
+  w':aead_writer i { w' == w }
+
+let wgetinfo #i (u: aead_writer i) =
+  if is_safe i then
+    dfst (u <: model_writer i)
+  else
+    u
+
+// JP: is this correct?
+let rgetinfo #_ u =
+  wgetinfo u
+
+let wlog #i w h =
+  B.deref h (dsnd (w <: model_writer i))
+
+let wfootprint #i w =
+  if is_safe i then
+    B.loc_addr_of_buffer (dsnd (w <: model_writer i))
+  else
+    B.loc_none
+
+let winvariant #i w h =
+  if is_safe i then
+    B.live h (dsnd (w <: model_writer i))
+  else
+    True
+
+let wframe_invariant #_ w h0 l h1 =
+  ()
+
+let frame_log #_ w h0 l h1 =
+  ()
+
+let gen i u =
+  if is_safe i then
+    let l: log #i u = Seq.empty #(entry i u) in
+    ((| u, B.malloc q_ae_region l 1ul |) <: model_writer i)
+  else
+    (u <: aead_writer i)
