src/Model.Flags.fsti
@@ -1,8 +1,22 @@
 module Model.Flags
 
-inline_for_extraction  val model : bool
+/// A generic flag that enables cryptographic modeling. Allows defining a switch
+/// between calling the specification / calling the implementation.
+inline_for_extraction
+val model : bool
+
 type ideal_flag = b:bool{b ==> model}
 
+/// Specific flags for each one of our cryptographic security assumptions.
+
+/// Ideal keying for transport secret (?)
 inline_for_extraction val ideal_TS: ideal_flag
+
+/// Ideal encrypted authenticated functionality
 inline_for_extraction val ideal_AEAD : f:ideal_flag{b2t f ==> b2t ideal_TS}
+
+/// Ideal PRF used with an auxiliary key.
+///
+/// TODO: figure out whether sequentialization is needed (e.g. because PRF needs
+/// a perfect random input from AEAD) or if it's just a stylistic thing
 inline_for_extraction val ideal_PRF : f:ideal_flag{b2t f ==> b2t ideal_AEAD}
