src/Model.Indexing.fsti
@@ -8,34 +8,40 @@ module AE = Spec.Agile.AEAD
 module HD = Spec.Hash.Definitions
 module G = FStar.Ghost
 
-let supported_hash = function
+let is_supported_hash = function
   | HD.SHA1 | HD.SHA2_256 | HD.SHA2_384 | HD.SHA2_512 -> true
   | _ -> false
 
-let supported_aead = function
+let is_supported_aead = function
   | AE.AES128_GCM | AE.AES256_GCM | AE.CHACHA20_POLY1305 -> true
   | _ -> false
 
-let supported_cipher = function
+let is_supported_cipher = function
   | C.AES128 | C.AES256 | C.CHACHA20 -> true
   | _ -> false
 
-type ha = a:HD.hash_alg{supported_hash a}
-type ea = a:AE.alg{supported_aead a}
-type ca = a:C.cipher_alg{supported_cipher a}
+type ha = a:HD.hash_alg{is_supported_hash a}
+type ea = a:AE.alg{is_supported_aead a}
+type ca = a:C.cipher_alg{is_supported_cipher a}
 
 val id: eqtype
-inline_for_extraction val is_honest: id -> bool
+inline_for_extraction
+val is_honest: id -> bool
+
 val id_ginfo: i:id -> GTot (ha * ea * ca)
 val id_info: i:id{model} -> a:(ha * ea * ca){a == id_ginfo i}
 
 val ae_id: eqtype
-inline_for_extraction val is_ae_honest: ae_id -> bool
+inline_for_extraction
+val is_ae_honest: ae_id -> bool
+
 val ae_id_ginfo: i:ae_id  -> GTot ea
 val ae_id_info: i:ae_id{model} -> a:ea{a == ae_id_ginfo i}
 
 val pne_id: eqtype
-inline_for_extraction val is_pne_honest: pne_id -> bool
+inline_for_extraction
+val is_pne_honest: pne_id -> bool
+
 val pne_id_ginfo: i:pne_id -> GTot ca
 val pne_id_info: i:pne_id{model} -> a:ca{a == pne_id_ginfo i}
 
